split unique indices

raft/proof/UniqueIndicesProof.v
@@ -11,27 +11,18 @@ Require Import Net.
 Require Import Raft.
 Require Import VerdiTactics.
 
-Require Import Sorted.
+Require Import SortedInterface.
 
 Require Import CommonTheorems.
+
+Require Import UniqueIndicesInterface.
 
 Section UniqueIndices.
   Context {orig_base_params : BaseParams}.
   Context {one_node_params : OneNodeParams orig_base_params}.
   Context {raft_params : RaftParams orig_base_params}.
 
-  Definition uniqueIndices_host_invariant net :=
-    (forall h, uniqueIndices (log (nwState net h))).
-
-  Definition uniqueIndices_nw_invariant net :=
-    forall p t leaderId prevLogIndex prevLogTerm entries leaderCommit,
-      In p (nwPackets net) ->
-      pBody p = AppendEntries t leaderId prevLogIndex prevLogTerm
-                              entries leaderCommit ->
-      uniqueIndices entries.
-    
-  Definition UniqueIndices net : Prop :=
-    uniqueIndices_host_invariant net /\ uniqueIndices_nw_invariant net.
+  Context {si : sorted_interface}.
 
   Theorem UniqueIndices_invariant :
     forall net,
@@ -45,5 +36,11 @@ Section UniqueIndices.
       eauto using sorted_uniqueIndices.
     - unfold uniqueIndices_nw_invariant, logs_sorted_nw in *.
       eauto using sorted_uniqueIndices.
+  Qed.
+
+  Instance uii : unique_indices_interface.
+  Proof.
+    split.
+    exact UniqueIndices_invariant.
   Qed.
 End UniqueIndices.
